New files: hvhdl/TransitionFacts.v, soundness/Soundness.v SoundnessDefs.v RisingEdgeFacts.v FallingEdgeFacts.v. These files carry some lemmas an defs about the proof of behavior preservation.

soundness/FallingEdgeFacts.v
@@ -1,250 +1,29 @@
-(** * Semantic Preservation Theorem *)
-
-Require Import NatMap.
+(** * Facts about Falling Edge and the Soundness Proof *)
 
 Require Import Coqlib.
-Require Import InAndNoDup.
-Require Import GlobalTypes.
 Require Import ListsPlus.
-Require Import SitpnSemanticsDefs.
+Require Import common.GlobalTypes.
 
-(* SITPN Libraries *)
-
-Require Import dp.SitpnTypes.
 Require Import dp.Sitpn.
-Require Import dp.SitpnSemantics.
+Require Import dp.SitpnSemanticsDefs.
 Require Import dp.Fired.
-
-(* H-VHDL Libraries *)
+Require Import dp.SitpnSemantics.
+Require Import dp.SitpnTypes.
 
 Require Import HVhdlTypes.
-Require Import Environment.
 Require Import SemanticalDomains.
-Require Import Simulation.
-Require Import CombinationalEvaluation.
-Require Import SynchronousEvaluation.
-Require Import DesignElaboration.
-Require Import AbstractSyntax.
+Require Import Environment.
 Require Import HilecopDesignStore.
-Require Import Initialization.
-Require Import Stabilize.
-Require Import PortMapEvaluation.
-
-(* SITPN to H-VHDL Libraries *)
+Require Import hvhdl.Stabilize.
+Require Import hvhdl.AbstractSyntax.
+Require Import hvhdl.CombinationalEvaluation.
+Require Import hvhdl.SynchronousEvaluation.
 
 Require Import GenerateHVhdl.
 
-(* Facts about NatMap. *)
-
-(** Defines the relation stating that an SITPN execution environment
-    and a H-VHDL design execution environment described the same
-    behavior.
-
-    - The environment [Ec] provides boolean values to the conditions
-    of [sitpn] depending on the cycle count [tau] 
-    
-    - The environment [Ep] provides values (must be boolean) to the input
-    ports of design [d] that implements the conditions of [sitpn].
-*)
-
-Definition EnvEq sitpn (Ec : nat -> C sitpn -> bool) (Ep : nat -> Clk -> IdMap value) : Prop := False.
-
-(** Defines the state similarity relation between an SITPN state and
-    a H-VHDL design state.
- *)
-
-Definition SimState {sitpn} (γ : P sitpn + T sitpn -> ident) (s : SitpnState sitpn) (σ : DState) : Prop :=
-
-  (* Markings are similar. *)
-  
-  forall (p : P sitpn) id__p σ__p,
-    (* [idp] is the identifier of the place component associated with
-       place [p] by the [γ] binder. *)
-    γ (inl p) = id__p ->
-
-    (* [σp] is the current state of component [idp] is the global design
-       state [σ]. *)
-    MapsTo id__p σ__p (compstore σ) ->
-
-    (* Marking of place [p] at state [s] equals value of signal
-       [s_marking] at state [σp]. *)
-    MapsTo Place.s_marking (Vnat (M s p)) (sigstore σ__p).
-
-Local Notation "γ ⊢ s '∼' σ" := (SimState γ s σ) (at level 50).
-
-(** States that two execution trace are similar. The first list
-    argument is the execution trace of an SITPN and the second list
-    argument is the execution trace of a VHDL design.
-    
-    By construction, and in order to be similar, the two traces must
-    have the same length, and must have pair-wise similar states. *)
-
-Inductive SimTrace {sitpn} γ : list (SitpnState sitpn) -> list DState -> Prop :=
-| SimTraceInit: SimTrace γ nil nil
-| SimTraceCons: forall s σ θ__s θ__σ,
-    γ ⊢ s ∼ σ ->
-    SimTrace γ θ__s θ__σ ->
-    SimTrace γ (s :: θ__s) (σ :: θ__σ).
-
-(** ** Rising edge marking equal lemma
-
-    States that starting from similar state, markings are equal
-    after the rising edge of the clock signal.  *)
-
-Lemma rising_edge_marking_equal :
-  forall Δ σ__r d θ σ' σ sitpn Ec τ s s' mm γ,
-
-    (* sitpn translates into d. *)
-    sitpn_to_hvhdl sitpn mm = Success d ->
-
-    (* Similar starting states *)
-    γ ⊢ s ∼ σ ->
-    
-    (* Rising edge from s to s', s ⇝↑ s' *)
-    SitpnStateTransition Ec τ s s' rising_edge -> 
-
-    (* Rising edge from σ to σr *)
-    vrising Δ σ (get_behavior d) σ__r -> 
-
-    (* Stabilize from σr to σ' *)
-    stabilize Δ σ__r (get_behavior d) θ σ' ->
-    
-    (* Conclusion *)
-    forall p id__p σ'__p,
-      (* [idp] is the identifier of the place component associated with
-       place [p] by the [γ] binder. *)
-      γ (inl p) = id__p ->
-
-      (* [σp] is the current state of component [idp] is the global design
-       state [σ]. *)
-      MapsTo id__p σ'__p (compstore σ') ->
-
-      (* Marking of place [p] at state [s] equals value of signal
-         [s_marking] at state [σp]. *)
-      MapsTo Place.s_marking (Vnat (@M sitpn s' p)) (sigstore σ'__p).
-Proof.
-Admitted.
-
-(** ** Rising edge states equal.
- 
-    Utopic lemma; not sure it is provable. *)
-
-Lemma rising_edge_states_equal :
-  forall Δ σ__r d θ σ' σ sitpn E__c τ s s' mm (γ : P sitpn + T sitpn -> ident),
-
-    (* sitpn translates into d. *)
-    sitpn_to_hvhdl sitpn mm = Success d ->
-
-    (* Similar starting states *)
-    γ ⊢ s ∼ σ ->
-    
-    (* Rising edge from s to s', s ⇝↑ s' *)
-    SitpnStateTransition E__c τ s s' rising_edge -> 
-
-    (* Rising edge from σ to σr *)
-    vrising Δ σ (get_behavior d) σ__r -> 
-
-    (* Stabilize from σr to σ' *)
-    stabilize Δ σ__r (get_behavior d) θ σ' ->
-    
-    (* Conclusion *)
-    γ ⊢ s' ∼ σ'.
-Proof.
-Admitted.
+Require Import SoundnessDefs.
 
 (** ** Falling edge compute fired lemma *)
-
-(*  *)
-
-(* All signals get a stable value at a certain point of the
-   stabilization trace. *)
-
-Lemma stable_value_signal :
-  forall θ Δ σ behavior σ',
-    stabilize Δ σ behavior θ σ' ->
-    forall s,
-      (exists v, MapsTo s v (sigstore σ)) ->
-      (exists θ' v,
-          (θ' <> [] \/ σ = σ') 
-          /\ LeListCons θ' θ 
-          /\ forall σ__j, List.In σ__j θ' -> MapsTo s v (sigstore σ__j)).
-Proof.
-  
-  induction 1; intros s Hx_sval.
-
-  (* BASE CASE *)
-  - exists nil.
-    inversion_clear Hx_sval as (v, Hmaps).
-    exists v.
-    split; [ right; reflexivity |
-             split; [apply LeListCons_refl |
-                     contradiction
-                    ]
-           ].
-
-  (* IND. CASE *)
-  - lazymatch goal with
-    | [ Hvcomb: vcomb _ _ _ _, H: (exists v, MapsTo s v (sigstore σ)) |- _ ] =>
-
-      (* s has a value at σ' *)
-      inversion_clear H as (v, Hmaps);
-        specialize (comb_maps_sigid Δ σ behavior σ' s v Hvcomb Hmaps) as Hex_v'
-    end.
-
-    specialize (IHstabilize s Hex_v').
-    inversion_clear IHstabilize as (θ', Hx); inversion_clear Hx as (v'', Hw).
-    decompose [and] Hw.
-
-    (* 2 CASES: θ' <> [] or σ' = σ'' *)
-    lazymatch goal with
-    | [ H: θ' <> [] \/ σ' = σ'' |- _ ] =>
-      inversion_clear H as [Hnotnil | Heq_σ']
-    end.
-
-    (* CASE θ' <> [] 
-       Instantiates θ' and v with the values coming from the IH, then trivial
-     *)
-    
-    + exists θ', v'';
-        split; [left; assumption |
-                split; [ apply LeListCons_cons; assumption | assumption]
-               ].
-
-    (* CASE σ' = σ''
-
-       Means that θ = [], otherwise contradicts the fact that σ' has
-       an empty event set. *)
-      
-    + lazymatch goal with
-      | [ H: stabilize _ _ _ _ _ |- _ ] =>
-        inversion H
-      end.
-
-      (* CASE θ = [] 
-         Then, there is but one non-empty trace θ' verifying
-         θ' <= [σ''], that is θ' = [σ'']
-       *)
-      -- exists [σ'']; inversion_clear Hex_v' as (v', Hmaps'); exists v'.
-         
-         (* Solves [σ''] <> [] \/ σ = σ'' *)
-         split; [ left; inversion 1 | auto].
-
-         (* Solves LeListCons [σ''] [σ''] *)
-         split; [ apply LeListCons_refl | auto].
-
-         (* Solves ∀ σj, σj ∈ [σ''] -> σj(s) = v' 
-            There's only one σj verifying σj ∈ [σ''].
-          *)
-         intros σ__j Hin; inversion_clear Hin as [Heq_σ'' | ];
-           [rewrite <- Heq_σ''; rewrite <- Heq_σ'; assumption |
-            contradiction].
-
-      (* CASE θ non-empty, then contradiction *)
-      -- lazymatch goal with
-         | [ H: events σ' <> _ |- _ ] =>
-           rewrite Heq_σ' in H; contradiction
-         end.
-Qed.
 
 (*  *)
 
@@ -278,9 +57,11 @@ Lemma stabilize_compute_auth :
       (* t ∈ sens(m) *)
       @Sens sitpn m t ->
 
-      forall s, exists θ' v,
-          LeListCons θ' θ 
-          /\ forall σ__j, List.In σ__j θ' -> MapsTo s v (sigstore σ__j) ->
+      (forall s, exists θ' v,
+          θ' <> []
+          /\ LeListCons θ' θ 
+          /\ forall σ__j, List.In σ__j θ' -> MapsTo s v (sigstore σ__j))
+      \/ σ = σ' ->
       
       (* Conclusion *)
       
@@ -392,7 +173,7 @@ Lemma elect_fired_compute_fired :
     
     (* Conclusion *)
     
-    forall m fired  tp m' fired',
+    forall m fired tp m' fired',
 
       (* All transitions of the fired list verify the conclusion *)
       (forall t,
@@ -406,6 +187,7 @@ Lemma elect_fired_compute_fired :
       
       MarkingSubPreSum (fun t => List.In t fired) (M s') m ->
 
+      (* Elect transitions to be fired from the [tp] list *)
       @ElectFired sitpn s' m fired tp (m', fired') ->
       
       forall t,
@@ -523,7 +305,7 @@ Proof.
 
   (* IND. CASE *)
   - apply IHHfired_aux.
-
+    
     (* CASE incl in Tlist *)
     + admit.
 
@@ -688,184 +470,3 @@ Lemma falling_edge_states_equal :
     γ ⊢ s' ∼ σ'.
 Proof.
 Admitted.
-
-(** ** Step lemma
-    
-    States that starting from similar state, state are similar after
-    one execution cycle.
-
- *)
-
-Lemma step_lemma :
-  forall sitpn mm d s s' E__c σ σ' Δ Mg σ__e P__i τ γ,
-    
-    (* sitpn translates into d. *)
-    sitpn_to_hvhdl sitpn mm = Success d ->
-
-    (* Starting states are similar *)
-    γ ⊢ s ∼ σ ->
-
-    (* Δ, σ are the results of the elaboration of d. *)
-    edesign hdstore Mg d Δ σ__e ->
-    
-    (* One execution cycle for SITPN *)
-    
-    @SitpnCycle sitpn E__c τ s s' ->
-
-    (* One execution cycle for VHDL *)
-    simcycle P__i Δ τ σ (get_behavior d) σ' ->
-     
-    (* Final states are similar *)
-    γ ⊢ s' ∼ σ'.
-Proof.
-  intros *; intros Htransl Hsim Helab Hsitpn_cyc Hhdl_cyc.
-  unfold SitpnCycle in Hsitpn_cyc.
-  inversion_clear Hsitpn_cyc as (s__i & (Hrising, Hfalling)).
-  inversion_clear Hhdl_cyc as
-      (σ__injr, σ__r, σ__i, σ__injf, σ__f, σ'', θ, θ',
-       Hhdl_rising, Hstab_rising, Hhdl_falling, Hstab_falling, Hinj_rising, Hinj_falling).
-
-  (* Must prove s similar to σ after capture of input values on rising edge. 
-     Necessary premise to apply [rising_edge_states_equal].      
-   *)
-  cut (γ ⊢ s ∼ σ__injr); intros Hsim_injr.
-  specialize (rising_edge_states_equal
-           Δ σ__r d θ σ__i σ__injr sitpn E__c τ s s__i mm γ
-           Htransl Hsim_injr Hrising Hhdl_rising Hstab_rising); intros Heq_int_states.
-
-  (* Must prove s similar to σ after capture of input values on falling edge. 
-     Necessary premise to apply [falling_edge_states_equal].
-   *)
-  cut (γ ⊢ s__i ∼ σ__injf); intros Hsim_injf.
-  apply (falling_edge_states_equal Δ σ__f d θ' σ' σ__injf sitpn E__c τ s__i s' mm γ
-                                   Htransl Hsim_injf Hfalling Hhdl_falling Hstab_falling).
-  
-  - admit.
-  - admit.
-Admitted.
-
-(** ** Equal Initial States  *)
-
-Lemma init_states_sim :
-  forall sitpn mm d Mg Δ σ__e σ0 γ,
-    
-    (* sitpn translates into d. *)
-    sitpn_to_hvhdl sitpn mm = Success d ->
-
-    (* ed, dstate are the results of the elaboration of d. *)
-    edesign hdstore Mg d Δ σ__e ->
-
-    (* initialization d's state. *)
-    init Δ σ__e (get_behavior d) σ0 ->
-
-    (* init states are similar *)
-    γ ⊢ (s0 sitpn) ∼ σ0.
-Proof.
-  intros *; intros Htransl Helab Hinit.
-  inversion_clear Hinit as (σ, beh, σ', σ'', θ, Hruninit, Hstab).
-
-Admitted.
-  
-(** ** Simulation Lemma *)
-
-Lemma simulation_lemma :
-  
-  forall sitpn Ec τ s θ__s s',
-
-    (* From state s to state s' after τ execution cycles, and
-       producing trace θs. *)
-    SitpnExecute Ec s τ θ__s s' ->
-
-    forall d mm Ep Mg Δ σ__e θ__σ σ σ' γ,
-      
-    (* sitpn translates into d. *)
-    sitpn_to_hvhdl sitpn mm = Success d ->
-
-    (* Environments are similar. *)
-    EnvEq sitpn Ec Ep ->
-
-    (* Δ, σe are the results of the elaboration of d. *)
-    edesign hdstore Mg d Δ σ__e ->
-
-    (* States s and σ are similar; *)
-    γ ⊢ s ∼ σ ->
-    
-    (* From σ to σ' after τ execution cycles, producing trace θσ. *)
-    simloop Ep Δ σ (get_behavior d) τ θ__σ σ' ->
-
-    (* Conclusion *)
-    SimTrace γ θ__s θ__σ.
-Proof.
-  intros *; intros Hexec; dependent induction Hexec;
-  intros *; intros Htransl Henveq Helab Hsimstate Hsim.
-  
-  (* CASE tau = 0, trivial. *)
-  - inversion Hsim; apply SimTraceInit.
-
-  (* CASE tau > 0 *)
-  - inversion_clear Hsim as [ τ0 σ0 σ'0 θ0 Hcyc Hsiml |  ].
-    
-    (* Specializes the induction hypothesis, then apply the step lemma. *)
-    
-    specialize (IHHexec d mm Ep Mg Δ σ__e θ0 σ0 σ').
-    specialize (IHHexec γ Htransl Henveq Helab).
-
-    (* Then, we need a lemma stating that s' ∼ σ0. That is, state are
-       similar after one execution cycle. *)
-
-    specialize (step_lemma sitpn mm d s s' Ec σ σ0 Δ Mg σ__e Ep (S tau) γ
-                           Htransl Hsimstate Helab H Hcyc)
-      as Heq_state_cyc.
-
-    (* Solve the induction case. *)
-    apply (@SimTraceCons sitpn γ s' σ0 θ θ0);
-      [ assumption | apply (IHHexec Heq_state_cyc Hsiml)].
-Qed.
-
-(** ** Semantic Preservation Theorem *)
-
-Theorem sitpn2vhdl_sound :
-  forall sitpn E__c τ θ__s s' d Mg E__p σ' mm Δ σ__e σ0 θ__σ γ,
-      
-    (* sitpn translates into d. *)
-    sitpn_to_hvhdl sitpn mm = Success d ->
-
-    (* (* Environments are similar. *) *)
-    EnvEq sitpn E__c E__p ->
-
-    (* sitpn is in state s' after τ execution cycles and yields
-       exec. trace θs. *)
-    
-    SitpnExecute E__c (s0 sitpn) τ θ__s s' ->    
-    
-    (* Design elaboration *)
-    edesign hdstore Mg d Δ σ__e ->
-    
-    (* Initialization of design state *)
-    init Δ σ__e (get_behavior d) σ0 ->
-
-    (* Simulation of design *)
-    simloop E__p Δ σ0 (get_behavior d) τ θ__σ σ' ->
-    
-    (* ** Conclusion: exec. traces are equal. ** *)
-    SimTrace γ θ__s θ__σ.
-Proof.
-  intros.
-
-  lazymatch goal with
-  | [
-    Htransl: sitpn_to_hvhdl _ _ = Success _,
-    Henveq: EnvEq _ _ _,
-    Hsitpnexec: SitpnExecute _ _ _ _ _,
-    Helab: edesign _ _ _ _ _,
-    Hinit: init _ _ _ _,
-    Hsimloop: simloop _ _ _ _ _ _ _
-    |- _ ] =>
-    specialize (init_states_sim sitpn mm d Mg Δ σ__e σ0 γ Htransl Helab Hinit) as Hinit_eq;
-      apply (simulation_lemma
-               sitpn E__c τ (s0 sitpn) θ__s s' Hsitpnexec d mm E__p Mg Δ σ__e θ__σ σ0 σ' γ
-               Htransl Henveq Helab Hinit_eq Hsimloop)
-  end.
-
-Qed.
-    
