hvhdl/Stabilize.v
@@ -7,6 +7,7 @@
  *)
 
 Require Import Coqlib.
+Require Import NatMap.
 Require Import NatSet.
 Require Import Environment.
 Require Import AbstractSyntax.
@@ -87,4 +88,86 @@ Proof.
     assumption.
     assert (Hconsl : d :: θ <> nil) by inversion 1.
     apply (IHstabilize (last_cons_inv Hconsl Hlast)).
+Qed.
+
+(* All signals get a stable value at a certain point of the
+   stabilization trace. *)
+
+Lemma stable_value_signal :
+  forall θ Δ σ behavior σ',
+    stabilize Δ σ behavior θ σ' ->
+    (forall s,
+      (exists v, MapsTo s v (sigstore σ)) ->
+      (exists θ', θ' <> []
+                    /\ LeListCons θ' θ
+                    /\ exists v, forall σ__j, List.In σ__j θ' -> MapsTo s v (sigstore σ__j)))
+    \/ σ = σ'.
+Proof.
+  
+  induction 1.
+
+  (* BASE CASE *)
+  - right; reflexivity.
+
+  (* IND. CASE 
+     In that case, the left part of the disj. is true.
+   *)
+  - left; intros.
+    
+    lazymatch goal with
+    | [ Hvcomb: vcomb _ _ _ _, H: (exists v, MapsTo s v (sigstore σ)) |- _ ] =>
+
+      (* s has a value at σ' *)
+      inversion_clear H as (v, Hmaps);
+        specialize (comb_maps_sigid Δ σ behavior σ' s v Hvcomb Hmaps) as Hex_v'
+    end.
+
+    (* 2 CASES: θ' <> [] or σ' = σ'' *)
+    inversion_clear IHstabilize as [Hnotnil | Heq_σ'].
+
+    (* CASE θ' <> [] 
+       Instantiates θ' and v with the values coming from the IH, then trivial
+     *)
+    
+    + specialize (Hnotnil s Hex_v'); inversion_clear Hnotnil as (θ', Hw).
+      decompose [and] Hw.
+      exists θ'; split;
+        [ assumption |
+          split; [ apply LeListCons_cons; assumption | assumption]
+        ].
+
+    (* CASE σ' = σ''
+
+       Means that θ = [], otherwise contradicts the fact that σ' has
+       an empty event set. *)
+      
+    + lazymatch goal with
+      | [ H: stabilize _ _ _ _ _ |- _ ] =>
+        inversion H
+      end.
+
+      (* CASE θ = [] 
+         Then, there is but one non-empty trace θ' verifying
+         θ' <= [σ''], that is θ' = [σ'']
+       *)
+      -- exists [σ'']; inversion_clear Hex_v' as (v', Hmaps').
+         
+         (* Solves [σ''] <> [] *)
+         split; [ inversion 1 | auto].
+
+         (* Solves LeListCons [σ''] [σ''] *)
+         split; [ apply LeListCons_refl | auto].
+
+         (* Solves ∀ σj, σj ∈ [σ''] -> σj(s) = v' 
+            There's only one σj verifying σj ∈ [σ''].
+          *)
+         exists v'; intros σ__j Hin; inversion_clear Hin as [Heq_σ'' | ];
+           [rewrite <- Heq_σ''; rewrite <- Heq_σ'; assumption |
+            contradiction].
+
+      (* CASE θ non-empty, then contradiction *)
+      -- lazymatch goal with
+         | [ H: events σ' <> _ |- _ ] =>
+           rewrite Heq_σ' in H; contradiction
+         end.
 Qed.
