hvhdl/TransitionFacts.v
@@ -1,0 +1,46 @@
+(** * Facts about the H-VHDL Transition Component *)
+
+Require Import common.NatMap.
+Require Import common.Coqlib.
+
+Require Import hvhdl.AbstractSyntax.
+Require Import hvhdl.SemanticalDomains.
+Require Import Environment.
+Require Import hvhdl.Petri.
+Require Import hvhdl.Transition.
+Require Import hvhdl.SynchronousEvaluation.
+Require Import hvhdl.Stabilize.
+Require Import hvhdl.HilecopDesignStore.
+Require Import hvhdl.DesignElaboration.
+Require Import hvhdl.CombinationalEvaluation.
+Require Import hvhdl.HVhdlTypes.
+Require Import hvhdl.Initialization.
+
+Require Import soundness.SoundnessDefs.
+
+(** ** Facts about the Transition Component Behavior on Falling Edge *)
+
+(** ** Facts about the Transition Component Behavior on Stabilization *)
+
+Lemma s_fired_assign_on_init :
+  forall id__t tg tip top Δ σ σ',
+    vruninit Δ σ (cs_comp id__t transition_entid tg tip top) σ' ->
+    
+    forall b σ'__t b' Δ__t,
+      MapsTo id__t (Component Δ__t transition_behavior) Δ ->
+      MapsTo id__t σ'__t (compstore σ') ->
+      MapsTo s_firable (Vbool b) (sigstore σ'__t) ->
+      MapsTo s_priority_combination (Vbool b') (sigstore σ'__t) ->
+      MapsTo s_fired (Vbool (andb b b')) (sigstore σ'__t).
+Proof.
+  intros *;
+    intros Hruninit;
+    dependent induction Hruninit;
+    intros *;
+    intros H__Δ Hσ'__t Hs_firable Hs_prio_comb. 
+
+  - inversion_clear Hpast as [Hrising | Hfalling].
+    
+    + induction Hrising using PastSimRising_ind.
+      
+Admitted.
