soundness/RisingEdgeFacts.v
@@ -1,0 +1,85 @@
+(** * Facts about Rising Edge and the Soundness Proof *)
+
+Require Import common.NatMap.
+Require Import common.GlobalTypes.
+
+Require Import dp.Sitpn.
+Require Import dp.SitpnSemantics.
+Require Import dp.SitpnTypes.
+
+Require Import hvhdl.Environment.
+Require Import hvhdl.SemanticalDomains.
+Require Import hvhdl.Stabilize.
+Require Import hvhdl.AbstractSyntax.
+Require Import hvhdl.SynchronousEvaluation.
+Require Import hvhdl.HVhdlTypes.
+
+Require Import sitpn2hvhdl.GenerateHVhdl.
+
+Require Import SoundnessDefs.
+
+(** ** Rising edge marking equal lemma
+
+    States that starting from similar state, markings are equal
+    after the rising edge of the clock signal.  *)
+
+Lemma rising_edge_marking_equal :
+  forall Δ σ__r d θ σ' σ sitpn Ec τ s s' mm γ,
+
+    (* sitpn translates into d. *)
+    sitpn_to_hvhdl sitpn mm = Success d ->
+
+    (* Similar starting states *)
+    γ ⊢ s ∼ σ ->
+    
+    (* Rising edge from s to s', s ⇝↑ s' *)
+    SitpnStateTransition Ec τ s s' rising_edge -> 
+
+    (* Rising edge from σ to σr *)
+    vrising Δ σ (get_behavior d) σ__r -> 
+
+    (* Stabilize from σr to σ' *)
+    stabilize Δ σ__r (get_behavior d) θ σ' ->
+    
+    (* Conclusion *)
+    forall p id__p σ'__p,
+      (* [idp] is the identifier of the place component associated with
+       place [p] by the [γ] binder. *)
+      γ (inl p) = id__p ->
+
+      (* [σp] is the current state of component [idp] is the global design
+       state [σ]. *)
+      MapsTo id__p σ'__p (compstore σ') ->
+
+      (* Marking of place [p] at state [s] equals value of signal
+         [s_marking] at state [σp]. *)
+      MapsTo Place.s_marking (Vnat (@M sitpn s' p)) (sigstore σ'__p).
+Proof.
+Admitted.
+
+(** ** Rising edge states equal.
+ 
+    Utopic lemma; not sure it is provable. *)
+
+Lemma rising_edge_states_equal :
+  forall Δ σ__r d θ σ' σ sitpn E__c τ s s' mm (γ : P sitpn + T sitpn -> ident),
+
+    (* sitpn translates into d. *)
+    sitpn_to_hvhdl sitpn mm = Success d ->
+
+    (* Similar starting states *)
+    γ ⊢ s ∼ σ ->
+    
+    (* Rising edge from s to s', s ⇝↑ s' *)
+    SitpnStateTransition E__c τ s s' rising_edge -> 
+
+    (* Rising edge from σ to σr *)
+    vrising Δ σ (get_behavior d) σ__r -> 
+
+    (* Stabilize from σr to σ' *)
+    stabilize Δ σ__r (get_behavior d) θ σ' ->
+    
+    (* Conclusion *)
+    γ ⊢ s' ∼ σ'.
+Proof.
+Admitted.
