soundness/Soundness.v
@@ -1,0 +1,222 @@
+(** * Semantic Preservation Theorem *)
+
+Require Import NatMap.
+
+Require Import Coqlib.
+Require Import InAndNoDup.
+Require Import GlobalTypes.
+Require Import ListsPlus.
+Require Import SitpnSemanticsDefs.
+
+(* SITPN Libraries *)
+
+Require Import dp.SitpnTypes.
+Require Import dp.Sitpn.
+Require Import dp.SitpnSemantics.
+Require Import dp.Fired.
+
+(* H-VHDL Libraries *)
+
+Require Import HVhdlTypes.
+Require Import Environment.
+Require Import SemanticalDomains.
+Require Import Simulation.
+Require Import CombinationalEvaluation.
+Require Import SynchronousEvaluation.
+Require Import DesignElaboration.
+Require Import AbstractSyntax.
+Require Import HilecopDesignStore.
+Require Import Initialization.
+Require Import Stabilize.
+Require Import PortMapEvaluation.
+
+(* SITPN to H-VHDL Libraries *)
+
+Require Import GenerateHVhdl.
+
+(* Soundness definitions and lemmas *)
+
+Require Import SoundnessDefs.
+Require Import RisingEdgeFacts.
+Require Import FallingEdgeFacts.
+
+(** ** Step lemma
+    
+    States that starting from similar state, state are similar after
+    one execution cycle.
+
+ *)
+
+Lemma step_lemma :
+  forall sitpn mm d s s' E__c σ σ' Δ Mg σ__e P__i τ γ,
+    
+    (* sitpn translates into d. *)
+    sitpn_to_hvhdl sitpn mm = Success d ->
+
+    (* Starting states are similar *)
+    γ ⊢ s ∼ σ ->
+
+    (* Δ, σ are the results of the elaboration of d. *)
+    edesign hdstore Mg d Δ σ__e ->
+    
+    (* One execution cycle for SITPN *)
+    
+    @SitpnCycle sitpn E__c τ s s' ->
+
+    (* One execution cycle for VHDL *)
+    simcycle P__i Δ τ σ (get_behavior d) σ' ->
+     
+    (* Final states are similar *)
+    γ ⊢ s' ∼ σ'.
+Proof.
+  intros *; intros Htransl Hsim Helab Hsitpn_cyc Hhdl_cyc.
+  unfold SitpnCycle in Hsitpn_cyc.
+  inversion_clear Hsitpn_cyc as (s__i & (Hrising, Hfalling)).
+  inversion_clear Hhdl_cyc as
+      (σ__injr, σ__r, σ__i, σ__injf, σ__f, σ'', θ, θ',
+       Hhdl_rising, Hstab_rising, Hhdl_falling, Hstab_falling, Hinj_rising, Hinj_falling).
+
+  (* Must prove s similar to σ after capture of input values on rising edge. 
+     Necessary premise to apply [rising_edge_states_equal].      
+   *)
+  cut (γ ⊢ s ∼ σ__injr); intros Hsim_injr.
+  specialize (rising_edge_states_equal
+           Δ σ__r d θ σ__i σ__injr sitpn E__c τ s s__i mm γ
+           Htransl Hsim_injr Hrising Hhdl_rising Hstab_rising); intros Heq_int_states.
+
+  (* Must prove s similar to σ after capture of input values on falling edge. 
+     Necessary premise to apply [falling_edge_states_equal].
+   *)
+  cut (γ ⊢ s__i ∼ σ__injf); intros Hsim_injf.
+  apply (falling_edge_states_equal Δ σ__f d θ' σ' σ__injf sitpn E__c τ s__i s' mm γ
+                                   Htransl Hsim_injf Hfalling Hhdl_falling Hstab_falling).
+  
+  - admit.
+  - admit.
+Admitted.
+
+(** ** Equal Initial States  *)
+
+Lemma init_states_sim :
+  forall sitpn mm d Mg Δ σ__e σ0 γ,
+    
+    (* sitpn translates into d. *)
+    sitpn_to_hvhdl sitpn mm = Success d ->
+
+    (* ed, dstate are the results of the elaboration of d. *)
+    edesign hdstore Mg d Δ σ__e ->
+
+    (* initialization d's state. *)
+    init Δ σ__e (get_behavior d) σ0 ->
+
+    (* init states are similar *)
+    γ ⊢ (s0 sitpn) ∼ σ0.
+Proof.
+  intros *; intros Htransl Helab Hinit.
+  inversion_clear Hinit as (σ, beh, σ', σ'', θ, Hruninit, Hstab).
+
+Admitted.
+  
+(** ** Simulation Lemma *)
+
+Lemma simulation_lemma :
+  
+  forall sitpn Ec τ s θ__s s',
+
+    (* From state s to state s' after τ execution cycles, and
+       producing trace θs. *)
+    SitpnExecute Ec s τ θ__s s' ->
+
+    forall d mm Ep Mg Δ σ__e θ__σ σ σ' γ,
+      
+    (* sitpn translates into d. *)
+    sitpn_to_hvhdl sitpn mm = Success d ->
+
+    (* Environments are similar. *)
+    EnvEq sitpn Ec Ep ->
+
+    (* Δ, σe are the results of the elaboration of d. *)
+    edesign hdstore Mg d Δ σ__e ->
+
+    (* States s and σ are similar; *)
+    γ ⊢ s ∼ σ ->
+    
+    (* From σ to σ' after τ execution cycles, producing trace θσ. *)
+    simloop Ep Δ σ (get_behavior d) τ θ__σ σ' ->
+
+    (* Conclusion *)
+    SimTrace γ θ__s θ__σ.
+Proof.
+  intros *; intros Hexec; dependent induction Hexec;
+  intros *; intros Htransl Henveq Helab Hsimstate Hsim.
+  
+  (* CASE tau = 0, trivial. *)
+  - inversion Hsim; apply SimTraceInit.
+
+  (* CASE tau > 0 *)
+  - inversion_clear Hsim as [ τ0 σ0 σ'0 θ0 Hcyc Hsiml |  ].
+    
+    (* Specializes the induction hypothesis, then apply the step lemma. *)
+    
+    specialize (IHHexec d mm Ep Mg Δ σ__e θ0 σ0 σ').
+    specialize (IHHexec γ Htransl Henveq Helab).
+
+    (* Then, we need a lemma stating that s' ∼ σ0. That is, state are
+       similar after one execution cycle. *)
+
+    specialize (step_lemma sitpn mm d s s' Ec σ σ0 Δ Mg σ__e Ep (S τ) γ
+                           Htransl Hsimstate Helab H Hcyc)
+      as Heq_state_cyc.
+
+    (* Solve the induction case. *)
+    apply (@SimTraceCons sitpn γ s' σ0 θ θ0);
+      [ assumption | apply (IHHexec Heq_state_cyc Hsiml)].
+Qed.
+
+(** ** Semantic Preservation Theorem *)
+
+Theorem sitpn2vhdl_sound :
+  forall sitpn E__c τ θ__s s' d Mg E__p σ' mm Δ σ__e σ0 θ__σ γ,
+      
+    (* sitpn translates into d. *)
+    sitpn_to_hvhdl sitpn mm = Success d ->
+
+    (* (* Environments are similar. *) *)
+    EnvEq sitpn E__c E__p ->
+
+    (* sitpn is in state s' after τ execution cycles and yields
+       exec. trace θs. *)
+    
+    SitpnExecute E__c (s0 sitpn) τ θ__s s' ->    
+    
+    (* Design elaboration *)
+    edesign hdstore Mg d Δ σ__e ->
+    
+    (* Initialization of design state *)
+    init Δ σ__e (get_behavior d) σ0 ->
+
+    (* Simulation of design *)
+    simloop E__p Δ σ0 (get_behavior d) τ θ__σ σ' ->
+    
+    (* ** Conclusion: exec. traces are equal. ** *)
+    SimTrace γ θ__s θ__σ.
+Proof.
+  intros.
+
+  lazymatch goal with
+  | [
+    Htransl: sitpn_to_hvhdl _ _ = Success _,
+    Henveq: EnvEq _ _ _,
+    Hsitpnexec: SitpnExecute _ _ _ _ _,
+    Helab: edesign _ _ _ _ _,
+    Hinit: init _ _ _ _,
+    Hsimloop: simloop _ _ _ _ _ _ _
+    |- _ ] =>
+    specialize (init_states_sim sitpn mm d Mg Δ σ__e σ0 γ Htransl Helab Hinit) as Hinit_eq;
+      apply (simulation_lemma
+               sitpn E__c τ (s0 sitpn) θ__s s' Hsitpnexec d mm E__p Mg Δ σ__e θ__σ σ0 σ' γ
+               Htransl Henveq Helab Hinit_eq Hsimloop)
+  end.
+
+Qed.
+    
