soundness/SoundnessDefs.v
@@ -1,0 +1,157 @@
+(** * Soundness Proof Definitions *)
+
+(* Common libraries *)
+
+Require Import common.Coqlib.
+
+(* SITPN Libraries *)
+
+Require Import dp.SitpnTypes.
+Require Import dp.Sitpn.
+
+(* H-VHDL Libraries *)
+
+Require Import hvhdl.HVhdlTypes.
+Require Import hvhdl.Environment.
+Require Import hvhdl.AbstractSyntax.
+Require Import hvhdl.SemanticalDomains.
+Require Import hvhdl.HilecopDesignStore.
+Require Import hvhdl.DesignElaboration.
+Require Import hvhdl.SynchronousEvaluation.
+Require Import hvhdl.Initialization.
+Require Import hvhdl.Stabilize.
+
+(** Defines the relation stating that an SITPN execution environment
+    and a H-VHDL design execution environment described the same
+    behavior.
+
+    - The environment [Ec] provides boolean values to the conditions
+    of [sitpn] depending on the cycle count [tau] 
+    
+    - The environment [Ep] provides values (must be boolean) to the input
+    ports of design [d] that implements the conditions of [sitpn].
+*)
+
+Definition EnvEq sitpn (Ec : nat -> C sitpn -> bool) (Ep : nat -> Clk -> IdMap value) : Prop := False.
+
+(** Defines the state similarity relation between an SITPN state and
+    a H-VHDL design state.
+ *)
+
+Definition SimState {sitpn} (γ : P sitpn + T sitpn -> ident) (s : SitpnState sitpn) (σ : DState) : Prop :=
+
+  (* Markings are similar. *)
+  
+  forall (p : P sitpn) id__p σ__p,
+    (* [idp] is the identifier of the place component associated with
+       place [p] by the [γ] binder. *)
+    γ (inl p) = id__p ->
+
+    (* [σp] is the current state of component [idp] is the global design
+       state [σ]. *)
+    MapsTo id__p σ__p (compstore σ) ->
+
+    (* Marking of place [p] at state [s] equals value of signal
+       [s_marking] at state [σp]. *)
+    MapsTo Place.s_marking (Vnat (M s p)) (sigstore σ__p).
+
+Notation "γ ⊢ s '∼' σ" := (SimState γ s σ) (at level 50).
+
+(** States that two execution trace are similar. The first list
+    argument is the execution trace of an SITPN and the second list
+    argument is the execution trace of a VHDL design.
+    
+    By construction, and in order to be similar, the two traces must
+    have the same length, and must have pair-wise similar states. *)
+
+Inductive SimTrace {sitpn} γ : list (SitpnState sitpn) -> list DState -> Prop :=
+| SimTraceInit: SimTrace γ nil nil
+| SimTraceCons: forall s σ θ__s θ__σ,
+    γ ⊢ s ∼ σ ->
+    SimTrace γ θ__s θ__σ ->
+    SimTrace γ (s :: θ__s) (σ :: θ__σ).
+
+(** *** PastSim Relations
+
+    Defines a simulation trace as the trace that led to the current
+    state in parameter.
+
+    A simulation trace is always linked to a design (or its elaborated
+    version) and its corresponding behavior.
+
+    There are 4 possible past simulation traces; following
+    the definition order, the current state is reached after:
+
+    - a falling edge phase (PastSimFalling) 
+    - a stabilization phase following a rising edge (PastSimRisingStab)
+    - a rising edge phase (PastSimRising)
+    - a stabilization phase following a falling edge (PastSimFallingStab)
+        
+ *)
+
+Inductive PastSimFalling (D : IdMap design) (M : IdMap value) (d : design) (Δ : ElDesign) : list DState -> DState -> Prop :=
+  PastSimFalling_cons :
+    forall σ__e θ σ σ__f,
+      (* Side conditions *)
+      edesign D M d Δ σ__e -> 
+      
+      (* Premises *)
+      PastSimRisingStab D M d Δ θ σ ->
+      vfalling Δ σ (get_behavior d) σ__f ->
+
+      (* Conclusion *)
+      PastSimFalling D M d Δ (θ ++ [σ]) σ__f
+                     
+with PastSimRisingStab (D : IdMap design) (M : IdMap value) (d : design) (Δ : ElDesign) : list DState -> DState -> Prop :=
+| PastSimRisingStab_cons :
+    forall σ__e θ θ' σ σ',
+      (* Side conditions *)
+      edesign D M d Δ σ__e -> 
+      
+      (* Premises *)
+      PastSimRising D M d Δ θ σ ->
+      stabilize Δ σ (get_behavior d) θ' σ' ->
+
+      (* Conclusion *)
+      PastSimRisingStab D M d Δ (θ ++ [σ]) σ'
+                        
+with PastSimRising (D : IdMap design) (M : IdMap value) (d : design) (Δ : ElDesign) : list DState -> DState -> Prop :=
+  PastSimRising_cons :
+    forall σ__e θ σ σ__r,
+      (* Side conditions *)
+      edesign D M d Δ σ__e -> 
+      
+      (* Premises *)
+      PastSimFallingStab D M d Δ θ σ ->
+      vrising Δ σ (get_behavior d) σ__r ->
+
+      (* Conclusion *)
+      PastSimRising D M d Δ (θ ++ [σ]) σ__r
+                     
+with PastSimFallingStab (D : IdMap design) (M : IdMap value) (d : design) (Δ : ElDesign)  : list DState -> DState -> Prop :=
+| PastSimFallingStab_init :
+    forall σ__e σ0,
+      (* Side conditions *)
+      edesign D M d Δ σ__e -> 
+
+      (* Premises *)
+      init Δ σ__e (get_behavior d) σ0 ->
+
+      (* Conclusion *)
+      PastSimFallingStab D M d Δ [] σ0
+                         
+| PastSimFallingStab_cons :
+    forall σ__e θ θ' σ σ',
+      (* Side conditions *)
+      edesign D M d Δ σ__e -> 
+      
+      (* Premises *)
+      PastSimFalling D M d Δ θ σ ->
+      stabilize Δ σ (get_behavior d) θ' σ' ->
+
+      (* Conclusion *)
+      PastSimFallingStab D M d Δ (θ ++ [σ]) σ'.
+
+Scheme Induction for PastSimFalling Sort Prop.
+
+
